break out monad2.v

insert_time_by_construction.v
@@ -1,49 +1,10 @@
 Set Implicit Arguments.
 
-Require Import braun util.
+Require Import braun util monad2.
 Require Import Coq.Logic.JMeq Coq.Program.Wf.
 Require Import Arith Arith.Even Arith.Div2.
 Require Import Omega.
 Require Import Program.Syntax.
-
-Inductive time_of : nat -> Type := 
-  Time : forall n, time_of n.
-
-Definition C (s: Set) (n:nat) : Set := (s * time_of n)%type. 
-
-Definition bind A B n n' (xn: C A n) (y: A -> C B n'): C B (n+n') :=
-  match xn with
-    | (x,tn) =>
-      match tn in time_of n with
-        | Time n =>
-          match y x with
-            | (r,tn') =>
-              match tn' in time_of n' with
-                | Time n' =>
-                  (r,Time (n+n'))
-              end
-          end
-      end
-  end.
-
-Definition ret (A: Set) (x: A): C A 0 := (x,Time 0).
-
-Definition inc (A : Set) n (k : nat) (x : C A n) : C A (n+k) :=
-  match x with
-    | (v,tn) =>
-      match tn in time_of n with
-        | Time n =>
-          (v, Time (n+k))
-      end
-  end.
-
-(* Definition time := snd. *)
-
-Notation "x >>= y" := (bind x y) (at level 55).
-Notation "x >> y" := (bind x (fun _ => y)) (at level 30, right associativity).
-Notation "x <- y ; z" := (bind y (fun x : _ => z)) (at level 30, right associativity).
-Notation "++ k ; c" := (inc k c) (at level 30, right associativity).
-
 
 Program Fixpoint fl_log_S n {wf lt n} : nat :=
   match n with
