Makefile
@@ -28,5 +28,12 @@ util.vo: util.v
 monad.vo: monad.v
 	$(COQC) monad.v
 
+
+insert_time_by_construction.vo: insert_time_by_construction.v monad2.vo
+	$(COQC) insert_time_by_construction.v
+
+monad2.vo: monad.v
+	$(COQC) monad2.v
+
 clean:
 	rm -f *.vo *.glob
